Tweaks in Closure conversion relation, updated compat lemmas, concrete bounds not quite there

theories/L6_PCPS/Heap/closure_conversion.v
@@ -27,8 +27,8 @@ Section CC.
     Scope :|: (Funs \\ Scope) :|: (FromList FVs \\ (Scope :|: Funs)).
 
   (* The free-variable set of a closure converted *)
-  Definition FV_cc (Scope Funs : Ensemble var) (σ : var -> var) (Γ : var) :=
-    Scope :|: (image σ (Funs \\ Scope)) :|: [set Γ].
+  Definition FV_cc (Scope Funs : Ensemble var) (Γ : var) :=
+    Scope :|: (Funs \\ Scope) :|: [set Γ].
 
   (* Closure application *)
   Definition AppClo f t xs f' Γ :=
@@ -39,7 +39,6 @@ Section CC.
   Inductive project_var :
     Ensemble var -> (* Variables in the current scope *)
     Ensemble var -> (* Names of the functions in the current function block *)
-    (var -> var) -> (* renaming of function names *)
     cTag -> (* tag of the current environment constructor *)
     var -> (* The environment argument *)
     list var -> (* The environment *)
@@ -50,27 +49,26 @@ Section CC.
     Ensemble var -> (* The new free set *)
     Prop :=
   | Var_in_Scope :
-      forall Scope Funs f c Γ FVs S x,
+      forall Scope Funs c Γ FVs S x,
         x \in Scope ->
-        project_var Scope Funs f c Γ FVs S x x Hole_c S
+        project_var Scope Funs c Γ FVs S x x Hole_c S
   | Var_in_Funs :
-      forall Scope Funs f c Γ FVs S x,
+      forall Scope Funs c Γ FVs S x,
         ~ x \in Scope ->
         x \in Funs ->
-        project_var Scope Funs f c Γ FVs S x (f x) Hole_c S
+        project_var Scope Funs c Γ FVs S x x Hole_c S
   | Var_in_FVs :
-      forall Scope Funs f c Γ FVs S x y N,
+      forall Scope Funs c Γ FVs S x y N,
         ~ x \in Scope ->
         ~ x \in Funs -> 
         nthN FVs N = Some x ->
         y \in S ->
-        project_var Scope Funs f c Γ FVs S x y
+        project_var Scope Funs c Γ FVs S x y
                     (Eproj_c y c N Γ Hole_c) (S \\ [set y]).
   
   Inductive project_vars :
     Ensemble var -> (* Variables in the current scope *)
     Ensemble var -> (* Names of the functions in the current function block *)
-    (var -> var) -> (* renaming of function names *)
     cTag -> (* tag of the current environment constructor *)
     var -> (* The environment argument *)
     list var -> (* The free variables *)
@@ -81,38 +79,38 @@ Section CC.
     Ensemble var -> (* The new free set *)
     Prop :=
   | VarsNil :
-      forall Scope Funs f c Γ FVs S,
-        project_vars Scope Funs f c Γ FVs S [] [] Hole_c S
+      forall Scope Funs c Γ FVs S,
+        project_vars Scope Funs c Γ FVs S [] [] Hole_c S
   | VarsCons :
-      forall Scope Funs f c Γ FVs y y' ys ys' C1 C2 S1 S2 S3,
-        project_var Scope Funs f c Γ FVs S1 y y' C1 S2 ->
-        project_vars Scope Funs f c Γ FVs S2 ys ys' C2 S3 ->
-        project_vars Scope Funs f c Γ FVs S1 (y :: ys) (y' :: ys') (comp_ctx_f C1 C2) S3.
+      forall Scope Funs c Γ FVs y y' ys ys' C1 C2 S1 S2 S3,
+        project_var Scope Funs c Γ FVs S1 y y' C1 S2 ->
+        project_vars Scope Funs c Γ FVs S2 ys ys' C2 S3 ->
+        project_vars Scope Funs c Γ FVs S1 (y :: ys) (y' :: ys') (comp_ctx_f C1 C2) S3.
 
   Inductive make_closures :
     fundefs -> (* The function block *)
-    Ensemble var -> (* The free set *)
+    Ensemble var -> (* The FVS of the rest of the program *)
     var -> (* The environment variable *)
     exp_ctx -> (* The context that constructs the closures *)
-    (var -> var) -> (* The renaming *)
-    Ensemble var -> (* The new free set *)
     Prop :=
   | closures_Fnil :
-      forall Γ f S,
-        make_closures Fnil S Γ Hole_c f S
-  | closures_Fcons :
-      forall f f' xs t e B Γ C g g' S S',
-        make_closures B (S \\ [set f']) Γ C g S' ->
-        In _ S f' ->
-        f_eq (g {f ~> f'}) g' ->
-        make_closures (Fcons f t xs e B) S Γ
-                      (Econstr_c f clo_tag [f' ; Γ] C)
-                      g' S'.
+      forall Γ FV,
+        make_closures Fnil FV Γ Hole_c
+  | closures_Fcons_in_FV :
+      forall f xs t e B FV Γ C,
+        make_closures B FV Γ C ->
+        f \in FV ->
+        make_closures (Fcons f t xs e B) FV Γ
+                      (Econstr_c f clo_tag [f ; Γ] C)
+  | closures_Fcons_nin_FV :
+      forall f xs t e B FV Γ C,
+        make_closures B FV Γ C ->
+        ~ f \in FV ->
+        make_closures (Fcons f t xs e B) FV Γ C.
   
   Inductive Closure_conversion :
     Ensemble var -> (* Variables in the current scope *)
     Ensemble var -> (* Names of the functions in the current function block *)
-    (var -> var) -> (* renaming of function names *)
     cTag -> (* tag of the current environment constructor *)
     var -> (* The environment argument *)
     list var -> (* The free variables - need to be ordered *)
@@ -121,99 +119,97 @@ Section CC.
     exp_ctx -> (* The context that the output expression should be put in *)
     Prop :=
   | CC_Econstr :
-      forall Scope Funs f c Γ FVs S' S x ys ys' C C' t e e',
+      forall Scope Funs c Γ FVs S' S x ys ys' C C' t e e',
         (* Variables for projected vars should not shadow the variables in
          scope, i.e. Scope U σ[Funs] U { Γ } *)
-        Disjoint _ S (FV_cc Scope Funs f Γ) ->
-        project_vars Scope Funs f c Γ FVs S ys ys' C S' ->
+        Disjoint _ S (FV_cc Scope Funs Γ) ->
+        project_vars Scope Funs c Γ FVs S ys ys' C S' ->
         (* We do not care about ys'. Should never be accessed again so do not
          add them aτ the current scope *)
-        Closure_conversion (x |: Scope) Funs f c Γ FVs e e' C' ->
-        Closure_conversion Scope Funs f c Γ FVs (Econstr x t ys e)
+        Closure_conversion (x |: Scope) Funs c Γ FVs e e' C' ->
+        Closure_conversion Scope Funs c Γ FVs (Econstr x t ys e)
                            (Econstr x t ys' (C' |[ e' ]|)) C
   | CC_Ecase :
-      forall Scope Funs f c Γ FVs x x' C S S' pats pats',
-        Disjoint _ S (FV_cc Scope Funs f Γ) ->
-        project_var Scope Funs f c Γ FVs S x x' C S' ->
+      forall Scope Funs c Γ FVs x x' C S S' pats pats',
+        Disjoint _ S (FV_cc Scope Funs Γ) ->
+        project_var Scope Funs c Γ FVs S x x' C S' ->
         Forall2 (fun (pat pat' : cTag * exp) =>
                    (fst pat) = (fst pat') /\
                    exists C' e',
                      snd pat' = C' |[ e' ]| /\
-                     Closure_conversion Scope Funs f c Γ FVs (snd pat) e' C')
+                     Closure_conversion Scope Funs c Γ FVs (snd pat) e' C')
                 pats pats' ->
-        Closure_conversion Scope Funs f c Γ FVs (Ecase x pats) (Ecase x' pats') C
+        Closure_conversion Scope Funs c Γ FVs (Ecase x pats) (Ecase x' pats') C
   | CC_Eproj :
-      forall Scope Funs f c Γ FVs S S' x y y' C C' t N e e',
-        Disjoint _ S (FV_cc Scope Funs f Γ) ->
-        project_var Scope Funs f c Γ FVs S y y' C S' ->
-        Closure_conversion (x |: Scope) Funs f c Γ FVs e e' C' ->
-        Closure_conversion Scope Funs f c Γ FVs (Eproj x t N y e)
+      forall Scope Funs c Γ FVs S S' x y y' C C' t N e e',
+        Disjoint _ S (FV_cc Scope Funs Γ) ->
+        project_var Scope Funs c Γ FVs S y y' C S' ->
+        Closure_conversion (x |: Scope) Funs c Γ FVs e e' C' ->
+        Closure_conversion Scope Funs c Γ FVs (Eproj x t N y e)
                            (Eproj x t N y' (C' |[ e' ]|)) C
   | CC_Efun :
-      forall Scope Funs f f' c Γ c' Γ' FVs FVs' FVs'' B B' e e' C C' Ce S1 S1' S2 S2' S3,
+      forall Scope Funs c Γ c' Γ' FVs FVs' FVs'' B B' e e' C C' Ce S1 S1' S3,
         (* The environment contains all the variables that are free in B *)
         (occurs_free_fundefs B) <--> (FromList FVs') ->
         (* needed for cost preservation *)
         NoDup FVs' ->
         (* Project the FVs to construct the environment *)
-        Disjoint _ S1 (FV_cc Scope Funs f Γ) ->
-        project_vars Scope Funs f c Γ FVs S1 FVs' FVs'' C' S1' ->
+        Disjoint _ S1 (FV_cc Scope Funs Γ) ->
+        project_vars Scope Funs c Γ FVs S1 FVs' FVs'' C' S1' ->
         (* Γ' is the variable that will hold the record of the environment *)
-        Disjoint _ S3 ((name_in_fundefs B) :|: (FV_cc Scope Funs f Γ)) ->
+        Disjoint _ S3 ((name_in_fundefs B) :|: (FV_cc Scope Funs Γ)) ->
         In _ S3 Γ' ->
-        Disjoint _ S2 ((bound_var_fundefs B) :|: [set Γ'] :|: (FV_cc Scope Funs f Γ)) ->
-        make_closures B S2  Γ' C f' S2' ->
-        Closure_conversion_fundefs B f' c' FVs' B B' ->
-        Closure_conversion ((name_in_fundefs B) :|: Scope) Funs f c Γ FVs e e' Ce  ->
-        Closure_conversion Scope Funs f c Γ FVs (Efun B e)
+        make_closures B (occurs_free e)  Γ' C ->
+        Closure_conversion_fundefs B c' FVs' B B' ->
+        Closure_conversion ((name_in_fundefs B) :|: Scope) Funs c Γ FVs e e' Ce  ->
+        Closure_conversion Scope Funs c Γ FVs (Efun B e)
                            (Efun B' (C |[ Ce |[ e' ]| ]|)) (comp_ctx_f C' (Econstr_c Γ' c' FVs'' Hole_c))
   | CC_Eapp :
-      forall Scope Funs g c Γ FVs f f' f'' ft env' ys ys' C S S',
-        Disjoint _ S (FV_cc Scope Funs g Γ) ->
+      forall Scope Funs c Γ FVs f f' f'' ft env' ys ys' C S S',
+        Disjoint _ S (FV_cc Scope Funs Γ) ->
         (* Project the function name and the actual parameter *)
-        project_vars Scope Funs g c Γ FVs S (f :: ys) (f' :: ys') C S' ->
+        project_vars Scope Funs c Γ FVs S (f :: ys) (f' :: ys') C S' ->
         (* (* Project the actual parameters *) *)
         (* project_vars Scope Funs Γ FVs S1 ys ys' C2 S2 -> *)
         (* The name of the function pointer and the name of the environment
          should not shadow the variables in the current scope and the
          variables that where used in the projections *)
         In _ S' f'' -> In _ S' env' -> f'' <> env' ->
-        Closure_conversion Scope Funs g c Γ FVs (Eapp f ft ys) (AppClo f' ft ys' f'' env') C
+        Closure_conversion Scope Funs c Γ FVs (Eapp f ft ys) (AppClo f' ft ys' f'' env') C
   | CC_Eprim :
-      forall Scope Funs g c Γ FVs S S' x ys ys' C C' f e e',
-        Disjoint _ S (FV_cc Scope Funs g Γ) ->
-        project_vars Scope Funs g c Γ FVs S ys ys' C S' ->
-        Closure_conversion (x |: Scope) Funs g c Γ FVs e e' C' ->
-        Closure_conversion Scope Funs g c Γ FVs (Eprim x f ys e)
+      forall Scope Funs c Γ FVs S S' x ys ys' C C' f e e',
+        Disjoint _ S (FV_cc Scope Funs Γ) ->
+        project_vars Scope Funs c Γ FVs S ys ys' C S' ->
+        Closure_conversion (x |: Scope) Funs c Γ FVs e e' C' ->
+        Closure_conversion Scope Funs c Γ FVs (Eprim x f ys e)
                            (Eprim x f ys' (C' |[ e' ]|)) C
   | CC_Ehalt :
-      forall Scope Funs g c Γ FVs x x' C S S',
-        Disjoint _ S (FV_cc Scope Funs g Γ) ->
+      forall Scope Funs c Γ FVs x x' C S S',
+        Disjoint _ S (FV_cc Scope Funs Γ) ->
         (* Project the function name and the actual parameter *)
-        project_var Scope Funs g c Γ FVs S x x' C S' ->
-        Closure_conversion Scope Funs g c Γ FVs (Ehalt x) (Ehalt x') C
+        project_var Scope Funs c Γ FVs S x x' C S' ->
+        Closure_conversion Scope Funs c Γ FVs (Ehalt x) (Ehalt x') C
   with Closure_conversion_fundefs :
          fundefs -> (* The current block *)
-         (var -> var) -> (* renaming of function names *)
          cTag -> (* tag of the current environment constructor *)
          list var -> (* The environment *)
          fundefs -> (* Before cc *)
          fundefs -> (* After cc *)
          Prop :=
-       | CC_Fcons :
-           forall B g c Γ' FVs S Sf Sf' f t ys e e' Cf C defs defs',
+       | CC_Fccons :
+           forall B c Γ' FVs S f t ys e e' Cf C defs defs',
              (* The environment binding should not shadow the current scope
                (i.e. the names of the mut. rec. functions and the other arguments) *)
-             Disjoint _ S (image g (name_in_fundefs B) :|: (FromList ys) :|: (bound_var e)) ->
+             Disjoint _ S ((name_in_fundefs B) :|: (FromList ys) :|: (bound_var e)) ->
              In _ S  Γ' ->
-             make_closures B Sf Γ' Cf g Sf' -> 
-             Closure_conversion_fundefs B g c FVs defs defs' ->
-             Closure_conversion (FromList ys) (name_in_fundefs B) g c Γ' FVs e e' C ->
-             Closure_conversion_fundefs B g c FVs (Fcons f t ys e defs )
-                                        (Fcons (g f) t (Γ' :: ys) (Cf |[ (C |[ e' ]|) ]|) defs')
+             make_closures B ((occurs_free e) \\ FromList ys) Γ' Cf -> 
+             Closure_conversion_fundefs B c FVs defs defs' ->
+             Closure_conversion (FromList ys) (name_in_fundefs B) c Γ' FVs e e' C ->
+             Closure_conversion_fundefs B c FVs (Fcons f t ys e defs )
+                                        (Fcons f t (Γ' :: ys) (Cf |[ (C |[ e' ]|) ]|) defs')
        | CC_Fnil :
-           forall B g c FVs,
-             Closure_conversion_fundefs B g c FVs Fnil Fnil.
+           forall B c FVs,
+             Closure_conversion_fundefs B c FVs Fnil Fnil.
   
 
   (** * Computational defintion of closure conversion *)
